Translation/SLiftSubst.v
@@ -51,6 +51,7 @@ Fixpoint lift n k t : sterm :=
   | sProjT2 p => sProjT2 (lift n k p)
   | sProjTe p => sProjTe (lift n k p)
   | sSort s => sSort s
+  | sInd ind s => sInd ind s
   end.
 
 Notation lift0 n t := (lift n 0 t).
@@ -105,6 +106,7 @@ Fixpoint subst t k u :=
   | sProjT2 p => sProjT2 (subst t k p)
   | sProjTe p => sProjTe (subst t k p)
   | sSort s => sSort s
+  | sInd ind s => sInd ind s
   end.
 
 Notation subst0 t u := (subst t 0 u).
