Translation/XTyping.v
@@ -47,6 +47,11 @@ Inductive typing (Σ : global_context) : scontext -> sterm -> sterm -> Type :=
     Σ ;;; Γ |-x u : A ->
     Σ ;;; Γ |-x sRefl A u : sEq A u u
 
+| type_Ind Γ ind s :
+    wf Σ Γ ->
+    forall univs decl (isdecl : declared_inductive (fst Σ) ind univs decl),
+      Σ ;;; Γ |-x sInd ind s : sSort s
+
 | type_conv Γ t A B s :
     Σ ;;; Γ |-x t : A ->
     Σ ;;; Γ |-x B : sSort s ->
